<?xml version="1.0" encoding="UTF-8"?>

<rdf:RDF xmlns="http://www.coskey.org/owl/ontologies/crime/#"
         xmlns:bfo="http://www.ifomis.org/bfo/1.1"
         xmlns:bio="http://purl.org/vocab/bio/01"
         xmlns:dc="http://purl.org/dc/elements/1.1"
         xmlns:foaf="http://xmlns.com/foaf/0.1"
         xmlns:geo="http://www.w3.org/2003/01/geo/wgs84_pos#"
         xmlns:gfo="http://www.onto-med.de/ontologies/gfo.owl#"
         xmlns:gr="http://purl.org/goodrelations/v1"
         xmlns:owl="http://www.w3.org/2002/07/owl#"
         xmlns:owl-time="http://www.w3.org/2006/time#"
         xmlns:prov="http://www.w3.org/ns/prov#"
         xmlns:qo="http://purl.org/qual/qual-o"
         xmlns:rdf="http://www.w3.org/1999/02/22-rdf-syntax-ns#"
         xmlns:rdfs="http://www.w3.org/2000/01/rdf-schema#"
         xmlns:sem="http://semanticweb.cs.vu.nl/2009/11/sem/"
         xmlns:sioc="http://rdfs.org/sioc/spec"
         xmlns:ssn="http://purl.oclc.org/NET/ssnx/ssn"
         xmlns:trn="http://vocab.org/transit"
         xmlns:xsd="http://www.w3.org/2001/XMLSchema#"
         >

    <rdfs:comment>
      TODO: 
        xmlns:fhwa	
        xmlns:fibo
        xmlns:iao
        xmlns:ic
        xmlns:obo
        xmlns:trip
    </rdfs:comment>       

    <rdfs:comment>
      TODO: 
        owl:AnnotationProperty
        owl:ObjectProperty
        owl:Restriction

        owl:allValuesFrom
        owl:disjointWith
        owl:equivalentProperty
        owl:hasValue
        owl:intersectionOf
        owl:inverseOf
        owl:members
        owl:onProperty
        owl:someValuesFrom
        owl:unionOf

        rdf:Description

        rdf:type

        rdfs:domain
        rdfs:label
        rdfs:range
        rdfs:subClassOf
        rdfs:subPropertyOf
    </rdfs:comment>       

    <owl:Ontology rdf:about="">
        <rdfs:comment>
            Crime Ontology                           
            Author: Jay Coskey
        </rdfs:comment>
    </owl:Ontology>

     <owl:Class rdf:ID="Airplane">
          <rdfs:subClassOf rdf:resource="http://www.w3.org/2002/07/owl#Thing"/>
     </owl:Class>

     <owl:DatatypeProperty rdf:ID="modeOfTransportation">
          <rdfs:domain rdf:resource="#Money"/>
          <rdfs:range rdf:resource="http://www.w3.org/2001/XMLSchema#string"/>
     </owl:DatatypeProperty>
</rdf:RDF>

